\medskip

\begin{enumerate}
\setlength\itemsep{1em}
\item $\begin{aligned}[t]
    \dfrac{3}{4}-0,53+\dfrac{7}{25}&=\dfrac{3}{4}-\dfrac{53}{100}+\dfrac{7}{25}\\
    &=\dfrac{75}{100}-\dfrac{53}{100}+\dfrac{28}{100}\\
    &=\dfrac{75-53+28}{100}\\
    &=\dfrac{50}{100}\\
    &=\dfrac{1}{2}
\end{aligned}$
\item $\begin{aligned}[t]
    \dfrac{\sqrt{\dfrac{166}{4}-\dfrac{11}{2}}}{2^3}&=\dfrac{\sqrt{\dfrac{83}{2}-\dfrac{11}{2}}}{2^3}\\
    &=\dfrac{\sqrt{36}}{2^3}\\
    &=\dfrac{6}{8}\\
    &=\dfrac{3}{4}
\end{aligned}$
\item $\begin{aligned}[t]
\dfrac{4^2+(14-\sqrt{121})^2}{1+(4-\sqrt{16})}&=\dfrac{16+(14-11)^2}{1+(4-4)}\\
&=\dfrac{16+(3)^2}{1}\\
&=16+9\\
&=25
\end{aligned}$
\end{enumerate}